<section xml:id="Comparison_theorems">
  <title>Comparison Theorems</title>
  <p>
    Let <m>X</m> be a Riemannian manifold with the Riemannian metric <m>ds^2</m>.
    Let <m>\omega_1, \ldots, \omega_n</m> be one forms such that
    <me>
      d s^2 = \omega ^2_1 + \cdots + \omega ^2_n
    </me>.
  </p>
  <p>
    Then by the theorem of Cartan,
    there are one forms <m>\{ \omega_{ij} \}</m> with <m>\omega_{ij} = - \omega _{ji}</m>,
    called the connection forms, such that
    <me>
      \left\{ \begin{array}{ll} d \omega_i = - \omega_{ij} \wedge \omega_j \\ d \omega _{ij} = - \omega _{ik} \wedge \omega_{kj} + \frac{1}{2} R_{ij kl} \, \omega _k \wedge \omega _l \end{array}  \right.
    </me>.
  </p>
  <p>
    The tensor <m>R_{ij k l}</m> is called the curvature tensor of the Riemannian metric <m>d s^2</m>.
  </p>
  <p>
    Let <m>U \subset \mathbb{R} ^{n-1}</m> be an open set.
    Let <m>\eta _2 , \ldots, \eta _n</m> be smooth one forms on <m>U</m> such that
    <me>
      (ds^1)^2 = \eta ^2_2 + \cdots + \eta ^2_n
    </me>
    defines a Riemannian metric on <m>U</m>.
    Let <m>\theta _2, \ldots, \theta _n</m> be local coordinates of <m>U</m>.
    Let <m>f (r, \theta)</m> be a positive function on <m>\mathbb{R}^+ \times U</m>.
    Define a Riemannian metric
    <me>
      ds^2 = d r ^2 + f^2 (r, \theta) \sum ^n _{i=2} \eta ^2 _i
    </me>
    on <m>\mathbb{R} ^+ \times U</m>.
  </p>
  <p>
    Example of the above setting appears in the Euclidean metric under polar coordinates.
    For example, in <m>\mathbb{R} ^2</m>,
    the Euclidean metric can be written as
    <me>
      d s^2 = d r^2 + r ^2 d \theta^2
    </me>.
  </p>
  <p>
    For this particular example,
    of course, the curvature of the above metric is zero.
    We shall see that, even in the more general setting,
    certainly components of the curvature tensor appear to be quite simple.
  </p>
  <p>
    We let
    <md>
      <mrow>\omega_1 \amp  = \amp d r</mrow>
      <mrow>\omega_k \amp  = \amp f (t , \theta ) \eta_k</mrow>
    </md>
    for <m>k>1</m>.
    Then
    <me>
      d s^2 = \omega ^2_1 + \cdots +\omega ^2_n
    </me>.
  </p>
  <p>
    Let <m>e_1 , \ldots,
    e _n</m> be the dual basis of <m>\omega_1, \ldots, \omega_n</m>,
    and let <m>\eta_{kl}</m> be the connection form for <m>(ds^1)^2</m>.
    Define
    <md>
      <mrow>\omega_{1l} \amp  = \amp  - e _1 (\log f) \omega_l;</mrow>
      <mrow>\omega_{kl} \amp  = \amp  \eta _{kl} - e _k (\log f) \omega_l + e _l (\log f) \omega _k</mrow>
    </md>
    for <m>k , l > 1</m>.
    A straightforward computation gives
    <me>
      d \omega_i = - \omega_{ij} \wedge \omega_j
    </me>.
  </p>
  <p>
    Note that <m>e_1 = \frac{\partial }{\partial r}</m>.
    We claim that
    <me>
      d \omega _{1l} + \omega _{1k} \wedge \omega _{kl} = - \frac{e_k \left( \frac{\partial f}{\partial r} \right)}{f} \omega _k \wedge \omega _l
    </me>.
  </p>
  <p>
    Verification: Since
    <me>
      \omega _{1l} = - \frac{\partial }{\partial r} (lg f) \omega_l
    </me>,
    we have
    <me>
      d \omega _{1l} = - e _{k}  \left(\frac{\partial }{\partial r}( \log f)  \right) \omega _k \wedge \omega_l - \frac{\partial }{\partial r}( \log f)  d\omega_l
    </me>.
  </p>
  <p>
    On the other hand, we have
    <md>
      <mrow>\lefteqn{\omega_{1k} \wedge \omega_{kl} }</mrow>
      <mrow>\amp \amp  = -\frac{\partial }{\partial r}( \log f)   \omega_k \wedge \left( \eta _{kl} - {e}_k (\log f) \omega_l +    e _l (\log f) \omega _k \right)</mrow>
      <mrow>\amp   \amp = \frac{\partial }{\partial r}   d \eta_l +  \frac{\partial }{\partial r}( \log f)     e _k (\log f) \omega_k \wedge \omega_l </mrow>
    </md>.
  </p>
  <p>
    Since
    <me>
      {e} _m \left(\frac{\partial }{\partial r}  \log f\right)    = f^{-1} {e}_m \frac{\partial f}{\partial r}( \log f)    - { e}_m (\log f) \frac{\partial }{\partial r}( \log f)
    </me>,
    we have
    <me>
      d \omega _{1l} + \omega _{1k} \wedge \omega_{kl} = - \frac{{e}_m \left( \frac{\partial f}{\partial r} \right) }{f} \omega _m \wedge \omega_l
    </me>.
  </p>
  <p>
    The claim is proved.
    By the Cartan's formula, we have
    <me>
      R _{1l  m n} = - \delta _{ln}  \frac{{e}_m \left( \frac{\partial f}{\partial r} \right) }{f}  + \delta _{lm} \frac{{e}_n \left( \frac{\partial f}{\partial r} \right) }{f}
    </me>.
  </p>
  <p>
    The Ricci curvature at <m>\frac{\partial }{\partial r}</m> direction is
    <me>
      R_{11} = R_{1 l 1 l} = - (n-1) \frac{1}{f} \frac{\partial ^2 f}{\partial r^2}
    </me>.
  </p>
  <p>
    In general, A Riemannian metric under the polar coordinates can be written as
    <me>
      ds^2 = (dr)^2 + h _{ij} (r, \theta) d \theta _i d \theta_j
    </me>.
  </p>
  <p>
    In order to compute/estimate the curvature,
    we use Uhlenbeck's trick which we introduce now.
  </p>
  <p>
    Let <m>\omega _1 = dr</m> and <m>\omega _2 , \ldots, \omega_n</m> be defined such that
    <me>
      h_{ij} d \theta_i d \theta_j = \sum_{j > 1} \omega ^2 _j
    </me>.
  </p>
  <p>
    We write
    <me>
      \frac{\partial \omega _j}{\partial r} =\sum_{j>1} a_{ij} \omega _j
    </me>
    for <m>i>1</m> for some matrix valued function <m>(a_{ij})</m>.
    The Uhlenbeck's trick is that,
    by an orthogonal change of the co-frame,
    we can make <m>(a_{ij})</m> a symmetric matrix.
  </p>
  <p>
    To see this, we write the above equations into matrix form.
    Let
    <me>
      \omega = \left( \begin{array}{c} \omega_2 \\ \vdots\\ \omega_n \end{array} \right),   A = (a_{ij})
    </me>.
  </p>
  <p>
    Then
    <me>
      \frac{\partial \omega}{\partial r } = A \omega
    </me>.
  </p>
  <p>
    Let <m>A = B+C</m> be the decomposition of the matrix <m>A</m> into symmetric and skew-symmetric parts.
    Let <m>Q</m> be an orthogonal matrix-valued function.
    We solve the equation
    <me>
      \frac{\partial Q}{\partial r}    = - QC
    </me>
    with the initial value <m>Q(0)=I</m>.
    It is not hard to verify that <m>Q</m> are orthogonal matrices: we have
    <me>
      \frac{\partial (Q^TQ)}{\partial r}  = -\frac{\pa Q^T}{\pa r}Q+Q^T\frac{\pa Q}{\pa r}=0
    </me>
    using the differential equation and the fact that <m>C</m> is skew-symmetric.
  </p>
  <p>
    Changing the co-frame from <m>\omega</m> to <m>Q\omega</m>, we have
    <me>
      \frac{\pa}{\pa r}(Q\omega)=QBQ^T(Q\omega)
    </me>.
  </p>
  <p>
    Since <m>QBQ^T</m> is symmetric,
    up to an orthogonal change of the co-frame,
    we may assume thst the matrix <m>A</m> is symmetric.
    This proves the Uhlenbeck's trick.
  </p>
  <p>
    Now back to the computation of the curvature.
    Let <m>(\eta _{ij} )( i , j > 1)</m> be the connection forms of the Riemannian metric
    <me>
      h_{ij} d \theta _i d \theta _j
    </me>.
  </p>
  <p>
    Define
    <md>
      <mrow>\omega_{i1} \amp  = \amp  \frac{\partial \omega_i}{\partial r};</mrow>
      <mrow>\omega _{ij } \amp  = \amp \eta_{ij}</mrow>
    </md>
    for <m>i,j>1</m>.
    Then we have
    <me>
      d \omega _i = - \sum_{j=1}^n\omega_{ij} \wedge \omega_j
    </me>
    for <m>i > 1</m>.
    On the other hand, since <m>A</m> is symmetric, we have
    <me>
      \omega_{i1}\wedge\omega_i=0
    </me>.
  </p>
  <p>
    Therefore, <m>d\omega_1=0=-\omega_{1j}\wedge\omega_j</m>.
    Thus <m>(\omega_{ij})</m> is connection forms of <m>(ds)^2</m> with respect to the co-frame <m>(\omega_1,\cdots,\omega_n)</m>.
  </p>
  <p>
    We compute
    <me>
      d \omega _{i1} + \omega _{ik}  \wedge \omega _{k 1} = \frac{1}{2} R_{il  kl} \omega _k \wedge \omega _l
    </me>.
  </p>
  <p>
    If we only count the terms of the form
    <m>\{ d r \wedge \omega_i \}</m> in the above equation, we have
    <me>
      dr\wedge\frac{\pa w_{i1}}{\pa r}=R_{i11j}\omega_1\wedge\omega_j
    </me>.
  </p>
  <p>
    Thus we have
    <me>
      { Ric}\,\left(\frac{\pa}{\pa r}, \frac{\pa}{\pa r}\right)=R_{11}=\frac{\pa}{\pa r}\left(\sum_{i>1}a_{ii}\right) +\sum_{i,j>1}a_{ij}^2
    </me>.
  </p>
  <p>
    On the other hand, we have
    <me>
      \frac{\pa}{\pa r}(\omega_1\wedge\cdots\wedge\omega_n)=(\sum_{i>1} a_{ii})\omega_1\wedge\cdots\wedge\omega_n
    </me>.
  </p>
  <p>
    Therefore we have
    <me>
      {\partial\over \partial r} \sqrt{\det h_{ij}}  =\sum a_{ii}  \sqrt{\det h_{ij}}
    </me>.
  </p>
  <p>
    Using the Cauchy inequality, we have
    <men xml:id="x1">
      { Ric} \left( \frac{\partial }{\partial r}, \frac{\partial }{\partial r} \right) \geq\frac{\pa^2}{\pa r^2}\sqrt{\det h_{ij}}+\frac{1}{n-1}\left(\frac{\pa}{\pa r}\sqrt{\det h_{ij}}\right)^2
    </men>.
  </p>
  <p>
    Using the above computation, we get the following comparison theorem.
  </p>
  <theorem>
    <title>Laplacian comparison theorem</title>
    <statement>
      <p>
        Let <m>X</m> be a complete Riemannian manifold of dimension <m>n</m>.
        Let
        <me>
          { Ric} (X) \geq - (n - 1) K
        </me>.
      </p>
      <p>
        Let <m>N</m> be an <m>n</m>-dimensional simply connected space form of constant sectional curvature <m>-K</m>.
        Let <m>\rho_M, \rho_N</m> be the distance functions to fixed reference points,
        respectively.
        If <m>x \in X</m> and <m>y \in N</m> such that
        <me>
          \rho_M (x) = \rho _N (y)
        </me>.
      </p>
      <p>
        Then in the sense of distribution, we have
        <me>
          \Delta \rho _M (x) \leq \Delta \rho _N (y)
        </me>.
      </p>
    </statement>
  </theorem>
  <proof>
    <p>
      Outside the cut-locus and the reference points,
      the function <m>\rho_M</m> is smooth.
      Since <m>\rho_M</m> is the distance function,
      <me>
        |\nabla \rho_M|=1
      </me>.
    </p>
    <p>
      The Laplacian can be written as
      <me>
        \Delta_M = \frac{1}{\sqrt{g}} \frac{\partial }{\partial x_i} \left( g^{ij} \sqrt{g} \frac{\partial }{\partial x_j}\right)
      </me>.
    </p>
    <p>
      Under the assumption that
      <me>
        ds^2 = d\rho^2 +\sum_{i,j} h_{ij}\, d \theta_i d \theta_j
      </me>,
      we have
      <me>
        \Delta \rho = \frac{\partial f}{\partial r}
      </me>,
      where <m>f=\sqrt{\det h_{ij}}</m>.
      By <nbsp/><xref ref="x1"/>, we have
      <me>
        \frac{\partial^2 f}{\partial r^2} + \left( \frac{\partial f}{\partial r} \right) ^2 \geq - { Ric} \left( \frac{\partial }{\partial r} , \frac{\partial }{\partial r} \right)
      </me>.
    </p>
    <p>
      The corresponding function on <m>N</m> satisfies the <em>equality</em>
      <men xml:id="x2">
        \frac{\partial^2 f_0}{\partial r^2} + \left( \frac{\partial f_0}{\partial r} \right) ^2 = ( n-1) K
      </men>.
    </p>
    <p>
      If <m>r\to 0</m>, the asympototics <m>f</m> and <m>f_0</m> are
      <me>
        \frac{\partial f}{\partial r}  \sim \frac{n-1}{  r} ,  \;\;  \frac{\partial f_0}{\partial r} \sim  \frac{n-1}{\partial r}
      </me>.
    </p>
    <p>
      Since
      <me>
        - { Ric} \left(    \frac{\partial }{\partial r} ,  \frac{\partial }{\partial r}  \right) \leq ( n - 1) K
      </me>,
    </p>
    <p>
      By the maximum principle
      <me>
        \frac{\partial f}{\partial r}  \leq \frac{\partial f_0}{\partial r_0}
      </me>.
    </p>
    <p>
      This proves the comparison theorem at the smooth points of <m>f</m>.
    </p>
    <p>
      Solving the equation<nbsp/><xref ref="x2"/>, we get
      <me>
        f_0(r) = \frac{1}{\cosh \,  \sqrt K} \cdot \sinh \, \sqrt K r
      </me>.
    </p>
    <p>
      Thus we have
      <me>
        \Delta _N \rho = \frac{n-1}{\rho} k \rho \coth k\rho \leq \frac{n-1}{\rho}  (1 + k \rho)
      </me>.
    </p>
    <p>
      Thus the Laplacian comparison theorem can be written in the following more useful form:
      <me>
        \Delta _M \rho \leq \frac{n-1}{\rho} ( 1 + k \rho)
      </me>.
    </p>
    <p>
      We shall prove that the above inequality is true even at singular points of <m>\rho</m>,
      in the sense of distribution.
      To see this,
      we let <m>\Omega</m> be the domain in <m>X</m> such that <m>\rho</m> is smooth on <m>\Omega</m>.
      <m>\Omega</m> is a star-like domain in <m>X</m>.
      Apparently
      <me>
        X = \Omega \cup C u t (p)
      </me>
      where <m>Cut(p)</m> is the cut-locus of <m>X</m>.
      Since <m>\rho</m> is at least continuous,
      and since the measure of <m>Cut (p)</m> is zero, we must have
      <me>
        \int _X \rho \Delta \phi = \int _{\Omega}  \rho \Delta \phi
      </me>
      for any smooth function <m>\phi</m>.
      Let <m>\Omega _\varepsilon</m> be an exhaustion of <m>\Omega</m> in the sense that <m>\Omega _\varepsilon  \subset \Omega</m>.
      <m>\Omega _\varepsilon \subset \Omega  _{\varepsilon^{\prime}}</m> if <m>\varepsilon > \varepsilon ^\prime</m>, and
      <me>
        \lim_{\varepsilon \rightarrow 0} \Omega _\varepsilon = \Omega
      </me>.
    </p>
    <p>
      Then we have
      <md>
        <mrow>\int_X \rho \Delta \phi \amp  = \amp  - \int_X \nabla \rho \nabla \rho</mrow>
        <mrow>\amp  = \amp  \lim _{\varepsilon \rightarrow 0} (-1) \int _{ \Omega \varepsilon} \nabla \rho \nabla \phi </mrow>
      </md>.
    </p>
    <p>
      Using the Green's formula, we have
      <me>
        - \int _\Omega \nabla \rho \nabla \phi = \int _ \Omega \nabla u \cdot \phi - \int _{\partial \Omega \varepsilon } \phi \frac{\partial \rho}{\partial r}
      </me>.
    </p>
    <p>
      On the boundary <m>\partial \Omega \varepsilon</m>, we have
      <me>
        \frac{\partial \rho}{\partial r} \geq 0
      </me>.
    </p>
    <p>
      Thus we have
      <me>
        - \int _\Omega \nabla \rho \nabla \phi \leq \int _ {\Omega \varepsilon} \Delta  \rho \cdot \phi \leq   \int _{\Omega \varepsilon } \frac{n-1}{\rho }  ( 1+k\rho)\phi
      </me>
    </p>
    <p>
      Finally, we get
      <md>
        <mrow>\int_X \rho \nabla \phi  \amp  \leq \amp  \lim_{\varepsilon \rightarrow 0} \int _{\Omega \varepsilon} \frac{n-1}{\rho} ( 1 + k \rho) \phi</mrow>
        <mrow>\amp  = \amp  \int_X \frac{n-1}{\rho}(1+ k \rho) \phi</mrow>
      </md>
      which finishes the proof of the theorem.
    </p>
  </proof>
  <p>
    Using exactly the same method,
    we have the following volume comparison theorem of Bishop.
  </p>
  <theorem>
    <statement>
      <p>
        Let <m>X</m> be an <m>n</m>-dimensional complete Riemannian manifold.
        Let
        <me>
          { Ric}(X) \geq - (n-1) k^2
        </me>.
      </p>
      <p>
        Then
        <me>
          \frac{{ vol} \, \partial B(R)}{{ vol} _k \,( \partial B (R))} \downarrow
        </me>
        is a decreasing function.
      </p>
    </statement>
  </theorem>
  <corollary>
    <title>Bishop</title>
    <statement>
      <p>
        Let <m>X</m> be an <m>n</m>-dimensional Riemannian manifold.
        If <m>{ Ric} \geq (n-1) k</m>.
        Then for any <m>R > 0</m>
      </p>
    </statement>
  </corollary>
  <me>
    \frac{{ vol}\, (B_X (R))}{{ vol} (k, R)}
  </me>
  <p>
    is a decreasing function.
    In particular
    <me>
      { vol} B_X (R) \leq V (k, R)
    </me>
    where <m>V(k, R)</m> is the volume of ball of radius <m>R</m> in space form of curvature <m>k</m>.
  </p>
  <remark>
    <p>
      The Bochner formula gives another proof of <nbsp/><xref ref="x1"/>.
      Let <m>f</m> be a smooth function.
      Then we have
      <me>
        \frac{1}{2} \Delta |\nabla f| ^2 = |\nabla ^2 f |^2 + \frac{\partial }{\partial r} \Delta f + { Ric} ( \nabla  f, \nabla f )
      </me>.
    </p>
    <p>
      If we specialize <m>f</m> to be <m>r</m>,
      then <m>|\nabla r |^2 = 1</m> and <m>\Delta |\nabla r| ^2 \equiv 0</m>.
      On the other hand
      <me>
        | \nabla ^2 f |^2 \geq \sum_i f_{ii}^2 \geq \frac{1}{n-1} \left( \sum f_{ii} \right) ^2 = \frac{1}{n-1} ( \Delta f ) ^2
      </me>,
      and the inequality follows.
    </p>
  </remark>
  <remark>
    <p>
      The proof of the laplacian comparison theorem in this section is not that far away from the usual proof using the second variational formula of the geodesic distance.
      The fact that we can write the Riemannian metric in the form
      <me>
        dr^2 + h_{ij} d \theta_i d \theta_j
      </me>
      is ensured by the Gauss Lemma,
      which is proved by the first variational formula of the geodesic distance function.
    </p>
  </remark>
</section>