<section xml:id="Moser_iteration">
  <title>De Giorgi-Nash-Moser Estimates</title>
  <p>
    In classical Schauder estimates or <m>W^{2,p}</m> estimates,
    the continuity of the coefficients is required.
    Therefore, the methods are not usable in nonlinear case.
    In 1957, De Giorgi obtained the H&#xf6;lder estimate on elliptic equations of divergence form with
    <em>measurable</em> coefficients.
    In 1958, Nash independently got the similar estimates on parabolic equations.
    In 1960, Moser obtained a simplified proof and the Harnark inequality.
    These methods now becomes crucial in geometric analysis.
  </p>
  <p>
    We consider the following elliptic equation of divergence form:
    <men xml:id="div">
      -D_j(a^{ij}D_iu)+b^iD_i u+cu=0
    </men>
    such that
    <md>
      <mrow>\amp  \lambda|\xi|^2\leq a^{ij}\xi_i\xi_j\leq\Lambda|\xi|^2,\qquad \forall x\in\Omega,\,\xi\in\R^n</mrow>
      <mrow>\amp \sum_{i,j}||a^{ij}||_{L^\infty}+\sum_i||b^i||_{L^\infty}+||c||_{L^\infty}\leq\Lambda</mrow>
    </md>.
  </p>
  <p>
    For the sake of simplicity, we only consider the following equation
    <men xml:id="div-1">
      -D_j(a^{ij}D_iu)=0
    </men>.
  </p>
  <lemma>
    <statement>
      <p>
        Let <m>\phi(s)\in C_{loc}^{0,1}(\R)</m> be a convex function
        <ol>
          <li>
            <p>
              If <m>u</m> is<nbsp/><xref ref="div-1"/>'s weak subsolution,
              <m>\phi'(s)\geq 0</m>.
              Then <m>v=\phi(u)</m> is also a weak subsolution;
            </p>
          </li>
          <li>
            <p>
              If <m>u</m> is<nbsp/><xref ref="div-1"/>'s weak supersolution,
              <m>\phi'(s)\leq 0</m>.
              Then <m>v=\phi(u)</m> is also a weak subsolution.
            </p>
          </li>
        </ol>
      </p>
    </statement>
  </lemma>
  <p>
    \end{proof}
  </p>
  <lemma>
    <title>Local maximum principle</title>
    <statement>
      <p>
        Let <m>v\in H^{1,2}(B_R)</m> be a weak subsolution.
        Then for any <m>p>0</m>, <m>0\lt \theta\lt 1</m>, we have
        <me>
          \underset{{B_{\theta R}}}{ess\,sup}\, v\leq C\left(\fint_{B_R}(v^+)^p\right)^{1/p}
        </me>,
        where <m>C</m> only depends on <m>n</m>,
        <m>\Lambda/\lambda</m>, <m>p</m>,
        and <m>(1-\theta)^{-1}</m>.
      </p>
    </statement>
  </lemma>
  <p>
    \begin{proof} The lemma is true even if <m>v</m> is not bounded.
    However, for the sake of simplicity,
    we assume that <m>v</m> is essentially bounded.
  </p>
  <p>
    We first assume that <m>p\geq 2</m>.
    Since <m>v</m> is a weak subsolution, so is <m>v^+</m>.
    Thus we can assume that <m>v\geq 0</m>.
  </p>
  <p>
    For any testing function <m>\phi\geq 0</m>, we have
    <me>
      \int_{B_R} a^{ij}D_ivD_j\phi \leq 0
    </me>.
  </p>
  <p>
    We let <m>\xi\in C_0^\infty(B_R)</m> and <m>\phi=\xi^2v^{p-1}</m>.
    Then we have
    <me>
      (p-1)\int_{B_R}(a^{ij} D_i v D_j v)v^{p-2}\xi^2 dx \leq -2\int_{B_R}a^{ij} v^{p-1}\xi D_i v D_j\xi dx
    </me>.
  </p>
  <p>
    Thus there is a constant <m>C</m> such that
    <me>
      \int_{B_R}|D(\xi v^{p/2})|^2 dx\leq C\int_{B_R}|D\xi|^2v^p dx
    </me>.
  </p>
  <p>
    Using the Sobolev inequality, we have
    <me>
      \left(\int_{B_R}(\xi v^{p/2})^{2^*} dx\right)^{2/2^*}\leq C\int_{B_R}|D\xi|^2 v^p dx
    </me>,
    where
    <me>
      2^*=\frac{2n}{n-2}
    </me>.
  </p>
  <p>
    Let
    <me>
      R_k=R\left(\theta+\frac{1-\theta}{2^k}\right)
    </me>.
  </p>
  <p>
    Define <m>\xi_k\in C_0^\infty(B_{R_k})</m> such that
    <m>\xi_k\equiv 1</m> on <m>B_{R_{k+1}}</m>.
    Then
    <me>
      |D\xi_k|\leq\frac{2^{k+1}}{(1-\theta) R}
    </me>.
  </p>
  <p>
    Using this we have
    <me>
      \left(\int_{B_{R_{k+1}}}v^{\frac{np}{n-2}}dx\right)^{\frac{n-2}{n}}\leq\frac{C\cdot 4^k}{(1-\theta)^2R^2}\int_{B_{R_k}}v^p dx
    </me>.
  </p>
  <p>
    Thus we have
    <me>
      ||v||_{L^{\frac{np}{n-2}}}(B_{R_{k+1}})\leq (C\cdot 4^k)^{1/p}||v||_{L^p}(B_{R_k})
    </me>.
  </p>
  <p>
    We let
    <me>
      p_1=\frac{np}{n-2},\cdots, p_k=\left(\frac{n}{n-2}\right)^k p
    </me>.
  </p>
  <p>
    Then we have
    <me>
      ||v||_{L^{p_{k+1}}}(B_{R_{k+1}})\leq (C\cdot 4^k)^{1/p_k}||v||_{L^{p_k}}(B_{R_k})
    </me>.
  </p>
  <p>
    Since
    <me>
      \log\left(\prod_{k=1}^\infty (C\cdot 4^k)^{1/p_k}\right) =\sum_{k=1}^\infty\frac{1}{p_k}(\log C+k\log 4)\lt C
    </me>,
    there is a constant <m>C</m> such that
    <me>
      ||v||_{L^\infty}(B_{\theta R})\leq\frac{C}{((1-\theta)R)^{n/p}}\frac{1}{R^n}||v||_{L^p}(B_R)
    </me>.
  </p>
  <p>
    It remains to prove that the lemma is true for <m>0\lt p\lt 2</m>.
    To see this we first use the inequality for <m>p=2</m>.
    That is
    <me>
      \sup_{B_{\theta R}}\, v\leq\frac{C}{(1-\theta)^{n/2}}\left(\fint_{B_R}u^2\right)^{1/2}
    </me>.
  </p>
  <p>
    We have
    <me>
      \left(\int_{B_R}v^2\right)^{1/2}\leq\sup_{B_R}\, v^{1-p/2}\cdot\left(\int_{B_R}v^p\right)^{1/2}
    </me>.
  </p>
  <p>
    Using Young's inequality, we have
    <me>
      \phi(\theta R)=(1-\frac p2)\phi(R)+\frac{C}{((1-\theta)R)^{n/p}}||v||_{L^p}
    </me>,
    where
    <me>
      \phi(s)=\sup_{B_s}\, v
    </me>.
  </p>
  <p>
    Thus we have the inequality
    <me>
      \phi(t)\leq (1-\frac p2)\phi(s)+\frac{A}{(t-s)^\alpha}||v||_{L^p}
    </me>
    for any <m>t\geq s</m>.
    Let
    <me>
      t_0=R_0\lt R,\qquad t_{i+1}=t_i+(1-\tau)t^i(R-R_0)
    </me>
    and <m>0\lt \tau\lt 1</m> to be determined later.
    Then we have
    <me>
      \phi(t_i)\leq(1-\frac p2)\phi(t_{i+1})+\frac{A}{((1-\tau)t^i(R-R_0))^\alpha}||u||_{L^2}
    </me>.
  </p>
  <p>
    By iteration, we know that
    <me>
      \phi(R_0)\leq A||u||_{L^2}\frac{1}{((1-\tau)t^i(R-R_0))^\alpha} \left((1-\frac p2)\tau^\alpha+(1-\frac p2)^2\tau^{-2\alpha}+\cdots\right)
    </me>.
  </p>
  <p>
    We can choose <m>\tau</m> close to <m>1</m> such that <m>(1-p/2)t^{-\alpha}\lt 1</m>.
    Then the above sequence is convergent and the theorem is proved.
  </p>
  <lemma>
    <title>Weak Harnarck inequality</title>
    <statement>
      <p>
        Let <m>v</m> be the weak supersolution of<nbsp/><xref ref="div-1"/>.
        Then there is a <m>p_0>0</m> such that
        <me>
          \underset{B_{\theta R}}{{ ess}\,\inf}\, v\geq\frac{1}{C}\left(\fint_{B_R}v^{p_0} dx\right)^{1/p_0}
        </me>
      </p>
    </statement>
  </lemma>
  <proof>
    <p>
      We assume that <m>v>0</m> on <m>B_R</m>.
      Otherwise we can use <m>v+\eps</m> instead.
    </p>
    <p>
      Since <m>v</m> is a supersolution,
      <m>v^{-1}</m> is a subsolution.
      By the above lemma, we have
      <me>
        \underset{B_{\theta R}}{{ ess}\,\sup}\, v^{-p}\leq C\fint_{B_R} v^{-p} dx
      </me>,
      which is equivalent to
      <me>
        \underset{B_{\theta R}}{{ ess}\,\inf}\, v\geq C \left(\fint_{B_R} v^{-p} dx\right)^{-\frac 1p}
      </me>
    </p>
    <p>
      We write
      <md>
        <mrow>\amp \underset{B_{\theta R}}{{ ess}\,\inf}\, v\geq C \left(\fint_{B_R} v^{-p} dx\right)^{-\frac 1p}</mrow>
        <mrow>\amp =C\left(\fint_{B_R}v^{-p} dx\cdot\fint_{B_R}v^p dx\right)^{-1/p}\cdot\left(\fint_{B_R}v^p dx\right)^{1/p}</mrow>
      </md>.
    </p>
    <p>
      We just need to prove that there exists a <m>p_0>0</m> such that
      <me>
        \fint_{B_R}v^{-p} dx\cdot\fint_{B_R}v^p dx\leq C
      </me>.
    </p>
    <p>
      We let <m>w=\log v-\beta</m>,
      where <m>\beta</m> is a constant to be determined.
      We wish to prove that
      <men xml:id="wish">
        \int_{B_R}e^{p|w|} dx\leq C
      </men>
      for some <m>p>0</m>.
      If the above inequality is true then we have
      <me>
        \int_{B_R}e^{p\log v-p\beta} dx\leq C,\qquad \int_{B_R}e^{-p\log v+p\beta} dx\leq C
      </me>,
      and the lemma follows.
    </p>
    <p>
      The proof of <nbsp/><xref ref="wish"/> is somewhat complicated but the basic idea is still Moser iteration.
      Let <m>v^{-1}\xi^2</m> be a test function,
      where <m>\xi \in C_0^\infty(B_R)</m>, we have
      <me>
        0\geq\int a^{ij} v_i(v^{-1}\xi^2)_j=-\int \xi^2a^{ij}w_i w_j+2\int a^{ij} w_i \xi\xi_j
      </me>.
    </p>
    <p>
      Without loss of generality, we assume that <m>R=1</m>.
      Then we have
      <me>
        \int_{B_\sigma}|Dw|^2\leq C
      </me>
      for any <m>0\lt \sigma\lt 1</m>.
      By choosing suitable <m>\beta</m>,
      we have the Poincar&#xe9; inequality
      <me>
        \int_{B_\sigma}|w|^2 dx\leq C
      </me>.
    </p>
    <p>
      Let <m>\xi\in C_0^\infty(B_1)</m> and let <m>\phi=\xi^2|w|^{2q}</m>.
      Then we have
      <me>
        \int_{B_\sigma}\xi^2|w|^{2q}|D_i w|^2\leq 2q\int_{B_\sigma}\xi^2|w|^{2q-1} D_i w D_i|w|+2\int_{B_\sigma}\xi|w|^{2q}D_i wD_i \xi
      </me>.
    </p>
    <p>
      Using the Young's inequality, we have
      <me>
        2q|w|^{2q-1}\leq\frac{2q-1}{2q}|w|^{2q}+(2q)^{2q-1}
      </me>.
    </p>
    <p>
      Thus we have
      <me>
        \frac{1}{2q}\int_{B_\sigma}\xi^2|w|^{2q}|D_iw|^2\leq (2q)^{2q-1}\int_{B_\sigma}|D_i w|^2+4q\int_{B_\sigma}|w|^{2q}|D_i\xi|^2
      </me>.
    </p>
    <p>
      Finally, we get
      <me>
        \int_{B_\sigma}|D(\xi^2|w|^{2q})|^2 dx\leq C(2q)^{2q}+C\tau^{-2}q^2\int_{B_{\sigma+\tau}}|w|^{2q} dx
      </me>,
      where <m>C</m> only depends on <m>n</m>,
      <m>\Lambda/\lambda</m>, and <m>(1-\sigma)^{-1}</m>.
      Let <m>\kappa=n/(n-1)</m>.
      By Sobolev inequality, we have
      <me>
        \left(\int_{B_\sigma}|w|^{2q\kappa} dx\right)^{1/\kappa}\leq C(2q)^{2q}+C\tau^{-2}q^2\int_{B_{\sigma+\tau}}|w|^{2q} dx
      </me>.
    </p>
    <p>
      We let
      <me>
        q_i=\kappa^{i-1},\delta_0=\sigma, \delta_i=\delta_{i-1}-\frac{\sigma-1}{2^i}
      </me>
    </p>
    <p>
      Then
      <me>
        \left(\int_{B_{\delta_i}}|w|^{2\kappa^i} dx\right)^{1/\kappa} \leq C(\kappa)^{2(i-1)\kappa^{i-1}}+C(4\kappa)^i\int_{B_{\delta_{i-1}}}|w|^{2\kappa^{i-1}}dx
      </me>
    </p>
    <p>
      Let
      <me>
        I_j=\left(\int_{B_{\delta_j}}|w|^{2\kappa^j}\right)^{1/2\kappa^j}
      </me>.
    </p>
    <p>
      Then
      <me>
        I_i\leq C^{1/\kappa^{i-1}}\kappa^{i-1}+C^{1/\kappa^{i-1}}(4\kappa)^{i/\kappa^{i-1}}I_{i-1}
      </me>.
    </p>
    <p>
      Running the iteration we get
      <me>
        I_j\leq C\kappa^j+cI_0
      </me>.
    </p>
    <p>
      Thus we have
      <me>
        ||w||_{L^q(B_1)}\leq Cq
      </me>.
    </p>
    <p>
      If <m>pCe\lt 1</m>, then we must have
      <me>
        \int_{B_1}e^{p|w|}\leq C
      </me>.
    </p>
  </proof>
  <theorem>
    <title>Harnack Inequality</title>
    <statement>
      <p>
        Let <m>u</m> be a nonnegative solution of <nbsp/><xref ref="div-1"/>.
        Then we have
        <me>
          \underset{B_{\theta R}}{{ ess}\,\sup}\,u\leq C \underset{B_{\theta R}}{{ ess}\,\inf}\,u
        </me>
        where <m>C</m> only depends on <m>n, \lambda/\lambda, (1-\theta)^{-1}</m>.
      </p>
    </statement>
  </theorem>
  <theorem>
    <title>H&#xf6;lder estimate</title>
    <statement>
      <p>
        Using the above notations,
        <m>u</m> is H&#xf6;lder continuous in <m>B_{\theta R}</m>.
      </p>
    </statement>
  </theorem>
  <proof>
    <p>
      Let
      <me>
        M(R)=\underset{B_{\theta R}}{{ ess}\,\sup}\,u, m(R)=\underset{B_{\theta R}}{{ ess}\,\inf}\,u
      </me>.
    </p>
    <p>
      Let <m>w(R)=M(R)-m(R)</m>.
      Then
      <me>
        u-m(R)\geq 0
      </me>
      on <m>B_{\theta R}</m>.
      Thus
      <me>
        M(\theta R)-m(R)\leq C(m(\theta R)-m(R))
      </me>.
    </p>
    <p>
      Therefore
      <me>
        w(\theta R)\leq \left(1-\frac 1C\right)w(R)
      </me>
      hence
      <me>
        w(\theta^s R)\leq \left(1-\frac 1C\right)^sw(R)
      </me>.
    </p>
    <p>
      Let <m>R'\lt R</m>.
      Let <m>s</m> be such that
      <me>
        \theta^{s+1}R\leq R'\lt \theta^s R
      </me>.
    </p>
    <p>
      Then
      <me>
        w(R')\leq w(\theta^sR)\leq \left(1-\frac 1C\right)^sw(R)
      </me>.
    </p>
    <p>
      Since
      <me>
        s=\left[\frac{\log (R'/R)}{\log\theta}\right]-1
      </me>,
    </p>
    <p>
      We have
      <me>
        w(R')\leq\left(\frac{R'}{R}\right)^rw(R)
      </me>,
      where
      <me>
        r=\left(1-\frac 1C\right)^{(\log\theta)^{-1}}\lt 1
      </me>
    </p>
    <p>
      Let <m>x,y\in  B(\theta R)</m>.
      Then we have
      <me>
        |u(x)-u(y)|\leq C|x-y|^r
      </me>
      and the H&#xf6;lder continuity follows.
    </p>
  </proof>
</section>