<section xml:id="Poincare_Lemma">
  <title>The Poincar&#xe9; Lemma</title>
  <p>
    In this section, we prove the following
  </p>
  <theorem>
    <statement>
      <p>
        Let <m>U</m> be the unit ball of the original point of <m>\R^n</m>.
        Let <m>\omega</m> be a <m>p</m>-form on <m>U</m> with <m>p\geq 1</m>.
        Then there is a <m>p-1</m> form <m>\eta</m> such that <m>\omega=d\eta</m>.
      </p>
    </statement>
  </theorem>
  <proof>
    <p>
      If <m>\omega</m> is a <m>1</m>-form,
      the proof is straightforward.
      Let
      <me>
        f(x)=\int_{\ell}\omega
      </me>,
      where <m>\ell</m> is a curve connecting the original point to <m>x</m>.
      Then
      <me>
        df=\omega
      </me>.
    </p>
    <p>
      In general, we use the math induction.
      We write
      <me>
        \omega=\omega_1+dx_n\wedge\omega_2
      </me>,
      where <m>\omega_1,\omega_2</m> are forms without the factor <m>dx_n</m>.
      Let
      <me>
        \omega=\sum a_{i_1\cdots i_{p-1}}(x_1,\cdots,x_n)dx_{i_1}\wedge\cdots\wedge dx_{i_{p-1}}
      </me>.
    </p>
    <p>
      Define
      <me>
        \eta=\int a_{i_1\cdots i_{p-1}}(x_1,\cdots,x_n)dx_n\, dx_{i_1}\wedge\cdots\wedge dx_{i_{p-1}}
      </me>.
    </p>
    <p>
      Then <m>d(\omega-d\eta)=0</m> and
      <m>\omega-d\eta</m> has not <m>dx_n</m> factor.
      As a result, the coefficients of
      <m>\omega-d\eta</m> are independent to <m>x_n</m>.
      Thus the theorem follows from the inductive assumption.
    </p>
  </proof>
  <p>
    The following theorem is a nonlinear generalization of the above result:
  </p>
  <theorem>
    <statement>
      <p>
        Let <m>U</m> be the unit tube of the original point of <m>\R^n</m>.
        Let <m>\omega</m> is a skew-symmetric matrix valued <m>1</m>-form on <m>U</m>.
        Assume that
        <me>
          d\omega+\omega\wedge\omega=0
        </me>.
      </p>
      <p>
        Then on <m>U</m>, the equation
        <me>
          dg+\omega g=0
        </me>
        is solvable.
      </p>
    </statement>
  </theorem>
  <proof>
    <p>
      We assume that <m>g(0)=1</m>.
      Assume that for <m>r>0</m>,
      we can define <m>g(x_1,\cdots,x_r,0,\cdots,0)</m> such that
      <m>dg+\omega g=0</m> on <m>\{x_{r+1}=\cdots x_n=0\}</m>.
      We define <m>g(x_1,\cdots, x_{r+1},0,\cdots,0)</m> by the following ODE:
      <me>
        \left\{ \begin{array}{l} \frac{\pa g}{\pa x_{r+1}}+\omega_{r+1} g=0\\ g(x_1,\cdots,x_r,0,\cdots,0) \text{ were defined. } \end{array} \right.
      </me>
    </p>
    <p>
      To complete the proof,
      we need to prove that for any <m>k\leq r</m>, we have
      <men xml:id="b-1">
        \frac{\pa g}{\pa x_k}+\omega_k g=0
      </men>.
    </p>
    <p>
      Taking the derivative with respect to <m>x_{r+1}</m>, we get
      <me>
        \frac{\pa ^2 g}{\pa x_{r+1}\pa x_k}+\frac{\pa\omega_k}{\pa x_{r+1}}g+\omega_k\frac{\pa g}{\pa x_{r+1}}
      </me>.
    </p>
    <p>
      Using the ODE, we get
      <me>
        -\frac{\omega_{r+1}}{\pa x_k}g-\omega_{r+1}\frac{\pa g}{\pa x_k}+\frac{\pa\omega_k}{\pa x_{r+1}}g+\omega_k\frac{\pa g}{\pa x_{r+1}}
      </me>.
    </p>
    <p>
      Using the fact that <m>d\omega+\omega\wedge\omega=0</m>,
      we can prove that the expression in<nbsp/><xref ref="b-1"/> satisfies the ODE with the zero initial value,
      hence must be zero.
    </p>
  </proof>
</section>