<section xml:id="Reverse_holder">
  <title>The Reverse H&#xf6;lder Inequality</title>
  <p>
    In this section,
    we prove the classical Reverse H&#xf6;lder inequality of Gehring
    (cite gehring).
  </p>
  <p>
    Let <m>Q</m> be a tube in <m>\R^n</m>.
    Let <m>f(x)</m> be a measurable,
    bounded, and nonnegative function.
    Define the <em>maximum function</em> by
    <me>
      M(f, x)=\sup_{r>0}\,\fint_{B(x,r)} f(x) dx
    </me>.
  </p>
  <p>
    In this section, we shall prove
  </p>
  <theorem>
    <title>Reverse H&#xf6;lder Inequality</title>
    <statement>
      <p>
        Let <m>q>1</m> such that
        <me>
          (M(f^q,x))^{1/q}\leq b M(f,x)
        </me>
        a.e.
        <m>x</m>, where <m>b</m> is a constant.
        Then there is an <m>\eps=\eps(n,b,q)>0</m> such that
        <me>
          \fint_Q f^{q+\eps}(x) dx\leq C \left(\fint_Q f(x) dx\right)^{q+\eps}
        </me>.
      </p>
    </statement>
  </theorem>
  <p>
    By rescaling, we may assume that
    <men xml:id="x0">
      \fint_Q f^q(x) dx=1
    </men>.
  </p>
  <p>
    Define
    <me>
      E(t)=\{x\in Q\mid f(x)>t\}
    </me>.
  </p>
  <p>
    We first prove the following lemma
  </p>
  <lemma>
    <statement>
      <p>
        For all <m>t>1</m>, there is a constant <m>a=a(n,b,q)>0</m> such that
        <me>
          \int_{E(t)} f^q(x) dx\leq at^{q-1}\int_{E(t)} f(x) dx
        </me>.
      </p>
    </statement>
  </lemma>
  <proof>
    <p>
      Define
      <me>
        s=\alpha t
      </me>,
      where <m>\alpha>1</m> is a constant to be determined.
      By assumption
      <me>
        \fint_Q f^q(x) dx=1\leq s^q
      </me>.
    </p>
    <p>
      We use the function <m>f(x)</m> and the number <m>s^q</m> to perform the
      <em>Calder&#xf3;n-Zygmund decomposition</em>.
      We then define a sequence of cubes <m>Q_j\subset Q</m> such that
      <ol>
        <li>
          <p>
            each side of <m>Q_j</m> is parallel to a side of <m>Q</m>;
            the interior of <m>Q_j</m> are disjoint;
          </p>
        </li>
        <li>
          <p>
            <men xml:id="x1-1-a">
              s^q\lt \fint_{Q_j} f^q(x) dx\leq 2^n s^q
            </men>.
          </p>
        </li>
        <li>
          <p>
            for <em>a.e.</em> <m>x\not\in \bigcup_j Q_j</m>,
            we have <m>f(x)\leq s</m>.
          </p>
        </li>
      </ol>
    </p>
    <p>
      Briefly speaking,
      the sequences can be defined inductively in the following way:
      we first divide <m>Q</m> into <m>2^n</m> sub-cubes like in Figure (ref fig2)
    </p>
    <image>
<latex-image>
          <![CDATA[\begin{tikzpicture}\tkzInit[xmax=1,ymax=1,xmin=-1,ymin=-1]
   \tkzGrid
 \tkzText[above](0.5,0.1){\(Q'\)}\end{tikzpicture}]]>
</latex-image>
    </image>
    <p>
      Let <m>Q'</m> be one of the sub-cubes.
      Then
      <me>
        \fint_{Q'} f^q(x) dx\leq \frac{1}{m(Q')}\int_Q f^q(x)dx\leq 2^n s^q
      </me>.
    </p>
    <p>
      If
      <me>
        \fint_{Q'} f^q(x) dx>s^q
      </me>,
      we say <m>Q'</m> is
      <q>good</q>
      and we assign <m>Q'</m> as one of the <m>Q_j</m>'s.
      If <m>Q'</m> is not
      <q>good</q>, then since
      <me>
        \fint_{Q'} f^q(x) dx\leq s^q
      </me>,
      we can repeat the division as above.
      In this way,
      we get a sequence <m>\{Q_j\}</m> such that they satisfy <nbsp/><xref ref="x1-1-a"/>.
      Now for all <m>x\not\in \bigcup_j Q_j</m>,
      there is a sequence <m>Q_j''</m> shrinking to <m>x</m> such that
      <me>
        \fint_{Q_j''} f^q(x)dx\leq s^q
      </me>.
    </p>
    <p>
      Thus by the Lebesgue Theorem,
      for <em>a.e.</em> <m>x</m>, <m>f(x)\leq s</m>.
    </p>
    <p>
      We define
      <me>
        G=\bigcup_jQ_j
      </me>.
    </p>
    <p>
      Then we have
      <me>
        \int_{E(s)} f^q(x) dx=\int_G f^q(x)dx=\sum_j\int_{Q_j} f^q(x) dx\leq 2^n s^q m(G)
      </me>.
    </p>
    <p>
      On the other hand, let <m>x\in Q_j</m> and let <m>r={ diam}(Q_j)</m>.
      Then
      <me>
        \frac{1}{m(B(x,r))}\int_{B(x,r)} f^q(x) dx\geq \frac{1}{m(B(x,r))}\, m(Q_j) s^q\geq c_1 s^q
      </me>,
      where <m>c_1=c_1(n)>0</m> is a constant.
      By the definition of the maximum function, we have
      <me>
        M(f^q,x)\geq\fint_{B(x,r)} f^q(x) dx\geq c_1 s^q
      </me>.
    </p>
    <p>
      Thus by the assumption of the theorem, we have
      <me>
        M(f,x)\geq (c_1/b)^{1/q} s=(c_1/b)^{1/q} \alpha t>\beta t
      </me>.
    </p>
    <p>
      If we choose <m>\alpha</m> large enough,
      we can assume that <m>\beta>1</m>.
      By definition of the maximum function,
      for any <m>x</m>, there is an <m>r_x>0</m> such that
      <me>
        \fint_{B(x,r_x)} f(x)dx\geq \beta t
      </me>.
    </p>
    <p>
      Such a collection of balls <m>B(x,r_x)</m> covers <m>Q_j</m>.
      Thus by the Vitali Covering Theorem,
      there is a countable subset of balls <m>B_j</m> which are disjoint and the union of <m>5B_j</m> covers <m>Q</m>.
      We therefore have the inequality
      <me>
        m(G)\leq 5^n\sum_j m(B_j)
      </me>.
    </p>
    <p>
      Thus we have
      <me>
        \beta tm(B_j)\leq\int_{B_j} f(x) dx\leq\int_{B_j\cap E(t)} f(x) dx+tm(B_j)
      </me>.
    </p>
    <p>
      We therefore have
      <me>
        m(B_j)\leq\frac{1}{(\beta-1) t}\int_{B_j\cap E(t)} f(x) dx
      </me>.
    </p>
    <p>
      Thus we have
      <me>
        <md>
          \amp \int_{E(s)} f^q(x)dx\leq 2^n s^qm(G)\\ \amp \leq 10^n s^q\frac{1}{(\beta-1) t}\sum_j\int_{B_j\cap E(t)} f(x) dx\\\amp \leq 10^n s^q\frac{1}{(\beta-1) t}\int_{ E(t)} f(x) dx.
        </md>
      </me>
    </p>
    <p>
      On the other hand, we have
      <me>
        \int_{E(t)\backslash E(s)} f^q(x) dx\leq s^{q-1}\int_{E(t)} f(x) dx
      </me>.
    </p>
    <p>
      Combining the above two inequalities completes the proof of the lemma.
    </p>
  </proof>
  <proof>
    <p>
      Define
      <me>
        h(t)=\int_{E(t)} f(x) dx
      </me>.
    </p>
    <p>
      Then it is easy to verify that
      <me>
        \int_{E(t)} f^r(x) dx=-\int_t^\infty s^{r-1} dh(s)
      </me>.
    </p>
    <p>
      Thus the lemma can be written as
      <men xml:id="x2a">
        -\int_t^\infty s^{q-1} dh(s)\leq at^{q-1} h(t)
      </men>.
    </p>
    <p>
      Define
      <me>
        I(r)=-\int_1^\infty t^{r-1}dh(t)
      </me>.
      and for <m>p>q>0</m>, define
      <me>
        J=(p-q)\int_1^\infty t^{p-q-1}\left(-\int_t^\infty s^{q-1}dh(s)\right) dt
      </me>.
    </p>
    <p>
      Then by<nbsp/><xref ref="x2a"/>, we have
      <me>
        J\leq (p-q)\int_1^\infty at^{p-2} h(t) dt=\frac{a(p-q)}{p-1}\int_1^\infty h(t) dt^{p-1}= \frac{a(p-q)}{p-1}(-I(1)+I(p))
      </me>.
    </p>
    <p>
      On the other hand, we use integration by parts to get
      <me>
        J=\int_1^\infty\left(-\int_t^\infty s^{q-1}dh(s)\right)dt^{p-q}=I(p)-I(q)
      </me>.
    </p>
    <p>
      Thus we get
      <me>
        I(p)-I(q)\leq \frac{a(p-q)}{p-1}(-I(1)+I(p))
      </me>.
    </p>
    <p>
      Thus for <m>p</m> sufficiently close to <m>q</m>, we get
      <me>
        I(p)\leq C(I(q)+I(1))
      </me>.
    </p>
  </proof>
  <proof>
    <p>
      Since
      <me>
        \int_{E(t)}f^q(x)dx\leq at^{q-1}\int_{E(t)} f(x) dx
      </me>,
      for any <m>\eps>0</m>, we have
      <me>
        \int_1^\infty\left(t^{\eps-1}\int_{E(t)}f^q(x)dx\right) dt\leq a \int_1^\infty\left(t^{q-2+\eps}\int_{E(t)} f(x) dx \right)
      </me>.
    </p>
    <p>
      We have
      <me>
        <md>
          \amp LHS=\int_1^\infty\int_X t^{\eps-1}1_{\{f(x)>t\}}f^q(x) dxdt =\int_X\int_1^\infty t^{\eps-1}1_{\{f(x)>t\}}f^q(x) dtdx\\ \amp =\frac{1}{\eps}\int_X (f^{q+\eps}(x)-f^q(x))dx.
        </md>
      </me>
    </p>
    <p>
      Similarly, we have
      <me>
        RHS=\frac{a}{q-1+\eps}\int_X(f^{q+\eps}(x)-f^{q-1+\eps}(x))dx
      </me>.
    </p>
    <p>
      So the theorem is proved by assuming that <m>\eps>0</m> is sufficiently small.
    </p>
  </proof>
  <remark>
    <p>
      Note that the last inequality is not homogeneous, which is fine,
      because we normalize the integral into<nbsp/><xref ref="x0"/>.
    </p>
  </remark>
</section>